RocqOfRust/anza_xyz_solana_sdk/program_error/links/lib.v
@@ -1,0 +1,365 @@
+Require Import RocqOfRust.RocqOfRust.
+Require Import RocqOfRust.links.M.
+Require Import core.links.result.
+Require Import anza_xyz_solana_sdk.program_error.lib.
+
+Module ProgramError.
+  Inductive t : Set :=
+  | Custom (n : U32.t)
+  | InvalidArgument
+  | InvalidInstructionData
+  | InvalidAccountData
+  | AccountDataTooSmall
+  | InsufficientFunds
+  | IncorrectProgramId
+  | MissingRequiredSignature
+  | AccountAlreadyInitialized
+  | UninitializedAccount
+  | NotEnoughAccountKeys
+  | AccountBorrowFailed
+  | MaxSeedLengthExceeded
+  | InvalidSeeds
+  | BorshIoError
+  | AccountNotRentExempt
+  | UnsupportedSysvar
+  | IllegalOwner
+  | MaxAccountsDataAllocationsExceeded
+  | InvalidRealloc
+  | MaxInstructionTraceLengthExceeded
+  | BuiltinProgramsMustConsumeComputeUnits
+  | InvalidAccountOwner
+  | ArithmeticOverflow
+  | Immutable
+  | IncorrectAuthority
+  .
+
+  Global Instance IsLink : Link t := {
+    Φ := Ty.path "solana_program_error::ProgramError";
+    φ x :=
+      match x with
+      | Custom n =>
+          Value.StructTuple "solana_program_error::ProgramError::Custom" [] [] [φ n]
+      | InvalidArgument =>
+          Value.StructTuple "solana_program_error::ProgramError::InvalidArgument" [] [] []
+      | InvalidInstructionData =>
+          Value.StructTuple "solana_program_error::ProgramError::InvalidInstructionData" [] [] []
+      | InvalidAccountData =>
+          Value.StructTuple "solana_program_error::ProgramError::InvalidAccountData" [] [] []
+      | AccountDataTooSmall =>
+          Value.StructTuple "solana_program_error::ProgramError::AccountDataTooSmall" [] [] []
+      | InsufficientFunds =>
+          Value.StructTuple "solana_program_error::ProgramError::InsufficientFunds" [] [] []
+      | IncorrectProgramId =>
+          Value.StructTuple "solana_program_error::ProgramError::IncorrectProgramId" [] [] []
+      | MissingRequiredSignature =>
+          Value.StructTuple "solana_program_error::ProgramError::MissingRequiredSignature" [] [] []
+      | AccountAlreadyInitialized =>
+          Value.StructTuple "solana_program_error::ProgramError::AccountAlreadyInitialized" [] [] []
+      | UninitializedAccount =>
+          Value.StructTuple "solana_program_error::ProgramError::UninitializedAccount" [] [] []
+      | NotEnoughAccountKeys =>
+          Value.StructTuple "solana_program_error::ProgramError::NotEnoughAccountKeys" [] [] []
+      | AccountBorrowFailed =>
+          Value.StructTuple "solana_program_error::ProgramError::AccountBorrowFailed" [] [] []
+      | MaxSeedLengthExceeded =>
+          Value.StructTuple "solana_program_error::ProgramError::MaxSeedLengthExceeded" [] [] []
+      | InvalidSeeds =>
+          Value.StructTuple "solana_program_error::ProgramError::InvalidSeeds" [] [] []
+      | BorshIoError =>
+          Value.StructTuple "solana_program_error::ProgramError::BorshIoError" [] [] []
+      | AccountNotRentExempt =>
+          Value.StructTuple "solana_program_error::ProgramError::AccountNotRentExempt" [] [] []
+      | UnsupportedSysvar =>
+          Value.StructTuple "solana_program_error::ProgramError::UnsupportedSysvar" [] [] []
+      | IllegalOwner =>
+          Value.StructTuple "solana_program_error::ProgramError::IllegalOwner" [] [] []
+      | MaxAccountsDataAllocationsExceeded =>
+          Value.StructTuple "solana_program_error::ProgramError::MaxAccountsDataAllocationsExceeded" [] [] []
+      | InvalidRealloc =>
+          Value.StructTuple "solana_program_error::ProgramError::InvalidRealloc" [] [] []
+      | MaxInstructionTraceLengthExceeded =>
+          Value.StructTuple "solana_program_error::ProgramError::MaxInstructionTraceLengthExceeded" [] [] []
+      | BuiltinProgramsMustConsumeComputeUnits =>
+          Value.StructTuple "solana_program_error::ProgramError::BuiltinProgramsMustConsumeComputeUnits" [] [] []
+      | InvalidAccountOwner =>
+          Value.StructTuple "solana_program_error::ProgramError::InvalidAccountOwner" [] [] []
+      | ArithmeticOverflow =>
+          Value.StructTuple "solana_program_error::ProgramError::ArithmeticOverflow" [] [] []
+      | Immutable =>
+          Value.StructTuple "solana_program_error::ProgramError::Immutable" [] [] []
+      | IncorrectAuthority =>
+          Value.StructTuple "solana_program_error::ProgramError::IncorrectAuthority" [] [] []
+      end
+  }.
+
+  Definition of_ty : OfTy.t (Ty.path "solana_program_error::ProgramError").
+  Proof. eapply OfTy.Make with (A := t); reflexivity. Defined.
+  Smpl Add apply of_ty : of_ty.
+
+  Lemma of_value_with_Custom (n : U32.t) :
+    Value.StructTuple "solana_program_error::ProgramError::Custom" [] [] [φ n]
+    = φ (Custom n).
+  Proof. reflexivity. Qed.
+  Smpl Add apply of_value_with_Custom : of_value.
+  Definition of_value_Custom (n : U32.t) :
+    OfValue.t (Value.StructTuple "solana_program_error::ProgramError::Custom" [] [] [φ n]).
+  Proof. econstructor; apply of_value_with_Custom. Defined.
+  Smpl Add apply of_value_Custom : of_value.
+
+  Lemma of_value_with_InvalidArgument :
+    Value.StructTuple "solana_program_error::ProgramError::InvalidArgument" [] [] [] = φ InvalidArgument.
+  Proof. reflexivity. Qed.
+  Smpl Add apply of_value_with_InvalidArgument : of_value.
+  Definition of_value_InvalidArgument :
+    OfValue.t (Value.StructTuple "solana_program_error::ProgramError::InvalidArgument" [] [] []).
+  Proof. econstructor; apply of_value_with_InvalidArgument. Defined.
+  Smpl Add apply of_value_InvalidArgument : of_value.
+
+  Lemma of_value_with_InvalidInstructionData :
+    Value.StructTuple "solana_program_error::ProgramError::InvalidInstructionData" [] [] [] = φ InvalidInstructionData.
+  Proof. reflexivity. Qed.
+  Smpl Add apply of_value_with_InvalidInstructionData : of_value.
+  Definition of_value_InvalidInstructionData :
+    OfValue.t (Value.StructTuple "solana_program_error::ProgramError::InvalidInstructionData" [] [] []).
+  Proof. econstructor; apply of_value_with_InvalidInstructionData. Defined.
+  Smpl Add apply of_value_InvalidInstructionData : of_value.
+
+  Lemma of_value_with_InvalidAccountData :
+    Value.StructTuple "solana_program_error::ProgramError::InvalidAccountData" [] [] [] = φ InvalidAccountData.
+  Proof. reflexivity. Qed.
+  Smpl Add apply of_value_with_InvalidAccountData : of_value.
+  Definition of_value_InvalidAccountData :
+    OfValue.t (Value.StructTuple "solana_program_error::ProgramError::InvalidAccountData" [] [] []).
+  Proof. econstructor; apply of_value_with_InvalidAccountData. Defined.
+  Smpl Add apply of_value_InvalidAccountData : of_value.
+
+  Lemma of_value_with_AccountDataTooSmall :
+    Value.StructTuple "solana_program_error::ProgramError::AccountDataTooSmall" [] [] [] = φ AccountDataTooSmall.
+  Proof. reflexivity. Qed.
+  Smpl Add apply of_value_with_AccountDataTooSmall : of_value.
+  Definition of_value_AccountDataTooSmall :
+    OfValue.t (Value.StructTuple "solana_program_error::ProgramError::AccountDataTooSmall" [] [] []).
+  Proof. econstructor; apply of_value_with_AccountDataTooSmall. Defined.
+  Smpl Add apply of_value_AccountDataTooSmall : of_value.
+
+  Lemma of_value_with_InsufficientFunds :
+    Value.StructTuple "solana_program_error::ProgramError::InsufficientFunds" [] [] [] = φ InsufficientFunds.
+  Proof. reflexivity. Qed.
+  Smpl Add apply of_value_with_InsufficientFunds : of_value.
+  Definition of_value_InsufficientFunds :
+    OfValue.t (Value.StructTuple "solana_program_error::ProgramError::InsufficientFunds" [] [] []).
+  Proof. econstructor; apply of_value_with_InsufficientFunds. Defined.
+  Smpl Add apply of_value_InsufficientFunds : of_value.
+
+  Lemma of_value_with_IncorrectProgramId :
+    Value.StructTuple "solana_program_error::ProgramError::IncorrectProgramId" [] [] [] = φ IncorrectProgramId.
+  Proof. reflexivity. Qed.
+  Smpl Add apply of_value_with_IncorrectProgramId : of_value.
+  Definition of_value_IncorrectProgramId :
+    OfValue.t (Value.StructTuple "solana_program_error::ProgramError::IncorrectProgramId" [] [] []).
+  Proof. econstructor; apply of_value_with_IncorrectProgramId. Defined.
+  Smpl Add apply of_value_IncorrectProgramId : of_value.
+
+  Lemma of_value_with_MissingRequiredSignature :
+    Value.StructTuple "solana_program_error::ProgramError::MissingRequiredSignature" [] [] [] = φ MissingRequiredSignature.
+  Proof. reflexivity. Qed.
+  Smpl Add apply of_value_with_MissingRequiredSignature : of_value.
+  Definition of_value_MissingRequiredSignature :
+    OfValue.t (Value.StructTuple "solana_program_error::ProgramError::MissingRequiredSignature" [] [] []).
+  Proof. econstructor; apply of_value_with_MissingRequiredSignature. Defined.
+  Smpl Add apply of_value_MissingRequiredSignature : of_value.
+
+  Lemma of_value_with_AccountAlreadyInitialized :
+    Value.StructTuple "solana_program_error::ProgramError::AccountAlreadyInitialized" [] [] [] = φ AccountAlreadyInitialized.
+  Proof. reflexivity. Qed.
+  Smpl Add apply of_value_with_AccountAlreadyInitialized : of_value.
+  Definition of_value_AccountAlreadyInitialized :
+    OfValue.t (Value.StructTuple "solana_program_error::ProgramError::AccountAlreadyInitialized" [] [] []).
+  Proof. econstructor; apply of_value_with_AccountAlreadyInitialized. Defined.
+  Smpl Add apply of_value_AccountAlreadyInitialized : of_value.
+
+  Lemma of_value_with_UninitializedAccount :
+    Value.StructTuple "solana_program_error::ProgramError::UninitializedAccount" [] [] [] = φ UninitializedAccount.
+  Proof. reflexivity. Qed.
+  Smpl Add apply of_value_with_UninitializedAccount : of_value.
+  Definition of_value_UninitializedAccount :
+    OfValue.t (Value.StructTuple "solana_program_error::ProgramError::UninitializedAccount" [] [] []).
+  Proof. econstructor; apply of_value_with_UninitializedAccount. Defined.
+  Smpl Add apply of_value_UninitializedAccount : of_value.
+
+  Lemma of_value_with_NotEnoughAccountKeys :
+    Value.StructTuple "solana_program_error::ProgramError::NotEnoughAccountKeys" [] [] [] = φ NotEnoughAccountKeys.
+  Proof. reflexivity. Qed.
+  Smpl Add apply of_value_with_NotEnoughAccountKeys : of_value.
+  Definition of_value_NotEnoughAccountKeys :
+    OfValue.t (Value.StructTuple "solana_program_error::ProgramError::NotEnoughAccountKeys" [] [] []).
+  Proof. econstructor; apply of_value_with_NotEnoughAccountKeys. Defined.
+  Smpl Add apply of_value_NotEnoughAccountKeys : of_value.
+
+  Lemma of_value_with_AccountBorrowFailed :
+    Value.StructTuple "solana_program_error::ProgramError::AccountBorrowFailed" [] [] [] = φ AccountBorrowFailed.
+  Proof. reflexivity. Qed.
+  Smpl Add apply of_value_with_AccountBorrowFailed : of_value.
+  Definition of_value_AccountBorrowFailed :
+    OfValue.t (Value.StructTuple "solana_program_error::ProgramError::AccountBorrowFailed" [] [] []).
+  Proof. econstructor; apply of_value_with_AccountBorrowFailed. Defined.
+  Smpl Add apply of_value_AccountBorrowFailed : of_value.
+
+  Lemma of_value_with_MaxSeedLengthExceeded :
+    Value.StructTuple "solana_program_error::ProgramError::MaxSeedLengthExceeded" [] [] [] = φ MaxSeedLengthExceeded.
+  Proof. reflexivity. Qed.
+  Smpl Add apply of_value_with_MaxSeedLengthExceeded : of_value.
+  Definition of_value_MaxSeedLengthExceeded :
+    OfValue.t (Value.StructTuple "solana_program_error::ProgramError::MaxSeedLengthExceeded" [] [] []).
+  Proof. econstructor; apply of_value_with_MaxSeedLengthExceeded. Defined.
+  Smpl Add apply of_value_MaxSeedLengthExceeded : of_value.
+
+  Lemma of_value_with_InvalidSeeds :
+    Value.StructTuple "solana_program_error::ProgramError::InvalidSeeds" [] [] [] = φ InvalidSeeds.
+  Proof. reflexivity. Qed.
+  Smpl Add apply of_value_with_InvalidSeeds : of_value.
+  Definition of_value_InvalidSeeds :
+    OfValue.t (Value.StructTuple "solana_program_error::ProgramError::InvalidSeeds" [] [] []).
+  Proof. econstructor; apply of_value_with_InvalidSeeds. Defined.
+  Smpl Add apply of_value_InvalidSeeds : of_value.
+
+  Lemma of_value_with_BorshIoError :
+    Value.StructTuple "solana_program_error::ProgramError::BorshIoError" [] [] [] = φ BorshIoError.
+  Proof. reflexivity. Qed.
+  Smpl Add apply of_value_with_BorshIoError : of_value.
+  Definition of_value_BorshIoError :
+    OfValue.t (Value.StructTuple "solana_program_error::ProgramError::BorshIoError" [] [] []).
+  Proof. econstructor; apply of_value_with_BorshIoError. Defined.
+  Smpl Add apply of_value_BorshIoError : of_value.
+
+  Lemma of_value_with_AccountNotRentExempt :
+    Value.StructTuple "solana_program_error::ProgramError::AccountNotRentExempt" [] [] [] = φ AccountNotRentExempt.
+  Proof. reflexivity. Qed.
+  Smpl Add apply of_value_with_AccountNotRentExempt : of_value.
+  Definition of_value_AccountNotRentExempt :
+    OfValue.t (Value.StructTuple "solana_program_error::ProgramError::AccountNotRentExempt" [] [] []).
+  Proof. econstructor; apply of_value_with_AccountNotRentExempt. Defined.
+  Smpl Add apply of_value_AccountNotRentExempt : of_value.
+
+  Lemma of_value_with_UnsupportedSysvar :
+    Value.StructTuple "solana_program_error::ProgramError::UnsupportedSysvar" [] [] [] = φ UnsupportedSysvar.
+  Proof. reflexivity. Qed.
+  Smpl Add apply of_value_with_UnsupportedSysvar : of_value.
+  Definition of_value_UnsupportedSysvar :
+    OfValue.t (Value.StructTuple "solana_program_error::ProgramError::UnsupportedSysvar" [] [] []).
+  Proof. econstructor; apply of_value_with_UnsupportedSysvar. Defined.
+  Smpl Add apply of_value_UnsupportedSysvar : of_value.
+
+  Lemma of_value_with_IllegalOwner :
+    Value.StructTuple "solana_program_error::ProgramError::IllegalOwner" [] [] [] = φ IllegalOwner.
+  Proof. reflexivity. Qed.
+  Smpl Add apply of_value_with_IllegalOwner : of_value.
+  Definition of_value_IllegalOwner :
+    OfValue.t (Value.StructTuple "solana_program_error::ProgramError::IllegalOwner" [] [] []).
+  Proof. econstructor; apply of_value_with_IllegalOwner. Defined.
+  Smpl Add apply of_value_IllegalOwner : of_value.
+
+  Lemma of_value_with_MaxAccountsDataAllocationsExceeded :
+    Value.StructTuple "solana_program_error::ProgramError::MaxAccountsDataAllocationsExceeded" [] [] [] =
+    φ MaxAccountsDataAllocationsExceeded.
+  Proof. reflexivity. Qed.
+  Smpl Add apply of_value_with_MaxAccountsDataAllocationsExceeded : of_value.
+  Definition of_value_MaxAccountsDataAllocationsExceeded :
+    OfValue.t (Value.StructTuple "solana_program_error::ProgramError::MaxAccountsDataAllocationsExceeded" [] [] []).
+  Proof. econstructor; apply of_value_with_MaxAccountsDataAllocationsExceeded. Defined.
+  Smpl Add apply of_value_MaxAccountsDataAllocationsExceeded : of_value.
+
+  Lemma of_value_with_InvalidRealloc :
+    Value.StructTuple "solana_program_error::ProgramError::InvalidRealloc" [] [] [] = φ InvalidRealloc.
+  Proof. reflexivity. Qed.
+  Smpl Add apply of_value_with_InvalidRealloc : of_value.
+  Definition of_value_InvalidRealloc :
+    OfValue.t (Value.StructTuple "solana_program_error::ProgramError::InvalidRealloc" [] [] []).
+  Proof. econstructor; apply of_value_with_InvalidRealloc. Defined.
+  Smpl Add apply of_value_InvalidRealloc : of_value.
+
+  Lemma of_value_with_MaxInstructionTraceLengthExceeded :
+    Value.StructTuple "solana_program_error::ProgramError::MaxInstructionTraceLengthExceeded" [] [] [] =
+    φ MaxInstructionTraceLengthExceeded.
+  Proof. reflexivity. Qed.
+  Smpl Add apply of_value_with_MaxInstructionTraceLengthExceeded : of_value.
+  Definition of_value_MaxInstructionTraceLengthExceeded :
+    OfValue.t (Value.StructTuple "solana_program_error::ProgramError::MaxInstructionTraceLengthExceeded" [] [] []).
+  Proof. econstructor; apply of_value_with_MaxInstructionTraceLengthExceeded. Defined.
+  Smpl Add apply of_value_MaxInstructionTraceLengthExceeded : of_value.
+
+  Lemma of_value_with_BuiltinProgramsMustConsumeComputeUnits :
+    Value.StructTuple "solana_program_error::ProgramError::BuiltinProgramsMustConsumeComputeUnits" [] [] [] =
+    φ BuiltinProgramsMustConsumeComputeUnits.
+  Proof. reflexivity. Qed.
+  Smpl Add apply of_value_with_BuiltinProgramsMustConsumeComputeUnits : of_value.
+  Definition of_value_BuiltinProgramsMustConsumeComputeUnits :
+    OfValue.t (Value.StructTuple "solana_program_error::ProgramError::BuiltinProgramsMustConsumeComputeUnits" [] [] []).
+  Proof. econstructor; apply of_value_with_BuiltinProgramsMustConsumeComputeUnits. Defined.
+  Smpl Add apply of_value_BuiltinProgramsMustConsumeComputeUnits : of_value.
+
+  Lemma of_value_with_InvalidAccountOwner :
+    Value.StructTuple "solana_program_error::ProgramError::InvalidAccountOwner" [] [] [] = φ InvalidAccountOwner.
+  Proof. reflexivity. Qed.
+  Smpl Add apply of_value_with_InvalidAccountOwner : of_value.
+  Definition of_value_InvalidAccountOwner :
+    OfValue.t (Value.StructTuple "solana_program_error::ProgramError::InvalidAccountOwner" [] [] []).
+  Proof. econstructor; apply of_value_with_InvalidAccountOwner. Defined.
+  Smpl Add apply of_value_InvalidAccountOwner : of_value.
+
+  Lemma of_value_with_ArithmeticOverflow :
+    Value.StructTuple "solana_program_error::ProgramError::ArithmeticOverflow" [] [] [] = φ ArithmeticOverflow.
+  Proof. reflexivity. Qed.
+  Smpl Add apply of_value_with_ArithmeticOverflow : of_value.
+  Definition of_value_ArithmeticOverflow :
+    OfValue.t (Value.StructTuple "solana_program_error::ProgramError::ArithmeticOverflow" [] [] []).
+  Proof. econstructor; apply of_value_with_ArithmeticOverflow. Defined.
+  Smpl Add apply of_value_ArithmeticOverflow : of_value.
+
+  Lemma of_value_with_Immutable :
+    Value.StructTuple "solana_program_error::ProgramError::Immutable" [] [] [] = φ Immutable.
+  Proof. reflexivity. Qed.
+  Smpl Add apply of_value_with_Immutable : of_value.
+  Definition of_value_Immutable :
+    OfValue.t (Value.StructTuple "solana_program_error::ProgramError::Immutable" [] [] []).
+  Proof. econstructor; apply of_value_with_Immutable. Defined.
+  Smpl Add apply of_value_Immutable : of_value.
+
+  Lemma of_value_with_IncorrectAuthority :
+    Value.StructTuple "solana_program_error::ProgramError::IncorrectAuthority" [] [] [] = φ IncorrectAuthority.
+  Proof. reflexivity. Qed.
+  Smpl Add apply of_value_with_IncorrectAuthority : of_value.
+  Definition of_value_IncorrectAuthority :
+    OfValue.t (Value.StructTuple "solana_program_error::ProgramError::IncorrectAuthority" [] [] []).
+  Proof. econstructor; apply of_value_with_IncorrectAuthority. Defined.
+  Smpl Add apply of_value_IncorrectAuthority : of_value.
+
+  Module SubPointer.
+    Definition get_Custom_0 : SubPointer.Runner.t t
+      (Pointer.Index.StructTuple "solana_program_error::ProgramError::Custom" 0) :=
+    {|
+      SubPointer.Runner.projection x :=
+        match x with
+        | Custom n => Some n
+        | _ => None
+        end;
+      SubPointer.Runner.injection x y :=
+        match x with
+        | Custom _ => Some (Custom y)
+        | _ => None
+        end;
+    |}.
+
+    Lemma get_Custom_0_is_valid :
+      SubPointer.Runner.Valid.t get_Custom_0.
+    Proof.
+      constructor; intros; destruct a; try reflexivity; discriminate.
+    Qed.
+    Smpl Add apply get_Custom_0_is_valid : run_sub_pointer.
+  End SubPointer.
+End ProgramError.
+
+(* ProgramResult = Result<(), ProgramError> *)
+Module ProgramResult.
+  Definition t : Set := Result.t unit ProgramError.t.
+End ProgramResult.
