RocqOfRust/anza_xyz_solana_sdk/program_pack/links/lib.v
@@ -1,0 +1,61 @@
+Require Import RocqOfRust.RocqOfRust.
+Require Import RocqOfRust.links.M.
+Require Import anza_xyz_solana_sdk.program_error.links.lib.
+Require Import anza_xyz_solana_sdk.program_pack.lib.
+Require Import core.links.result.
+
+(*
+  pub trait Pack: Sealed + Sized {
+      const LEN: usize;
+      fn unpack_from_slice(src: &[u8]) -> Result<Self, ProgramError>;
+      fn pack_into_slice(&self, dst: &mut [u8]);
+
+      // Provided methods
+      fn get_packed_len() -> usize { ... }
+      fn unpack(input: &[u8]) -> Result<Self, ProgramError> { ... }
+      fn unpack_unchecked(input: &[u8]) -> Result<Self, ProgramError> { ... }
+      fn pack(src: Self, dst: &mut [u8]) -> Result<(), ProgramError> { ... }
+  }
+*)
+Module Pack.
+  Definition trait (Self : Set) `{Link Self} : TraitMethod.Header.t :=
+    ("solana_program_pack::Pack", [], [], Φ Self).
+
+  Definition Run_unpack (Self : Set) `{Link Self} : Set :=
+    TraitMethod.C (trait Self) "unpack" (fun method =>
+      forall (input : Ref.t Pointer.Kind.Ref (list U8.t)),
+        Run.Trait method [] [] [φ input] (Result.t Self ProgramError.t)
+    ).
+
+  Definition Run_unpack_unchecked (Self : Set) `{Link Self} : Set :=
+    TraitMethod.C (trait Self) "unpack_unchecked" (fun method =>
+      forall (input : Ref.t Pointer.Kind.Ref (list U8.t)),
+        Run.Trait method [] [] [φ input] (Result.t Self ProgramError.t)
+    ).
+
+  Definition Run_unpack_from_slice (Self : Set) `{Link Self} : Set :=
+    TraitMethod.C (trait Self) "unpack_from_slice" (fun method =>
+      forall (src : Ref.t Pointer.Kind.Ref (list U8.t)),
+        Run.Trait method [] [] [φ src] (Result.t Self ProgramError.t)
+    ).
+
+  Definition Run_pack (Self : Set) `{Link Self} : Set :=
+    TraitMethod.C (trait Self) "pack" (fun method =>
+      forall (src : Self) (dst : Ref.t Pointer.Kind.MutRef (list U8.t)),
+        Run.Trait method [] [] [φ src; φ dst] (Result.t unit ProgramError.t)
+    ).
+
+  Definition Run_pack_into_slice (Self : Set) `{Link Self} : Set :=
+    TraitMethod.C (trait Self) "pack_into_slice" (fun method =>
+      forall (self : Ref.t Pointer.Kind.Ref Self) (dst : Ref.t Pointer.Kind.MutRef (list U8.t)),
+        Run.Trait method [] [] [φ self; φ dst] unit
+    ).
+
+  Class Run (Self : Set) `{Link Self} : Set := {
+    unpack : Run_unpack Self;
+    unpack_unchecked : Run_unpack_unchecked Self;
+    unpack_from_slice : Run_unpack_from_slice Self;
+    pack : Run_pack Self;
+    pack_into_slice : Run_pack_into_slice Self;
+  }.
+End Pack.
