RocqOfRust/core/cell/links/mod.v
@@ -1,0 +1,70 @@
+Require Import RocqOfRust.RocqOfRust.
+Require Import RocqOfRust.links.M.
+Require Import core.cell.
+Require Import core.ops.links.deref.
+
+Module Ref.
+  Parameter t : forall (T : Set) `{Link T}, Set.
+
+  Parameter to_value : forall {T : Set} `{Link T}, t T -> Value.t.
+
+  Global Instance IsLink (T : Set) `{Link T} : Link (t T) := {
+    Φ := Ty.apply (Ty.path "core::cell::Ref") [] [Φ T];
+    φ := to_value;
+  }.
+
+  Definition of_ty T_ty :
+    OfTy.t T_ty ->
+    OfTy.t (Ty.apply (Ty.path "core::cell::Ref") [] [T_ty]).
+  Proof.
+    intros [T].
+    eapply OfTy.Make with (A := t T).
+    subst.
+    reflexivity.
+  Defined.
+  Smpl Add apply of_ty : of_ty.
+End Ref.
+
+(* impl<T: ?Sized> Deref for Ref<'_, T> *)
+Module Impl_Deref_for_Ref.
+  Instance run (T : Set) `{Link T} : Deref.Run (Ref.t T) T.
+  Admitted.
+End Impl_Deref_for_Ref.
+Export Impl_Deref_for_Ref.
+
+(* Approximation for core::cell::RefMut<T> *)
+Module RefMut.
+  Parameter t : forall (T : Set) `{Link T}, Set.
+
+  Parameter to_value : forall {T : Set} `{Link T}, t T -> Value.t.
+
+  Global Instance IsLink (T : Set) `{Link T} : Link (t T) := {
+    Φ := Ty.apply (Ty.path "core::cell::RefMut") [] [Φ T];
+    φ := to_value;
+  }.
+
+  Definition of_ty T_ty :
+    OfTy.t T_ty ->
+    OfTy.t (Ty.apply (Ty.path "core::cell::RefMut") [] [T_ty]).
+  Proof.
+    intros [T].
+    eapply OfTy.Make with (A := t T).
+    subst.
+    reflexivity.
+  Defined.
+  Smpl Add apply of_ty : of_ty.
+End RefMut.
+
+(* impl<T> Deref for RefMut<'_, T> *)
+Module Impl_Deref_for_RefMut.
+  Instance run (T : Set) `{Link T} : Deref.Run (RefMut.t T) T.
+  Admitted.
+End Impl_Deref_for_RefMut.
+Export Impl_Deref_for_RefMut.
+
+(* impl<T> DerefMut for RefMut<'_, T> *)
+Module Impl_DerefMut_for_RefMut.
+  Instance run (T : Set) `{Link T} : DerefMut.Run (RefMut.t T) T.
+  Admitted.
+End Impl_DerefMut_for_RefMut.
+Export Impl_DerefMut_for_RefMut.
