RocqOfRust/solana_program_token/interface/links/state.v
@@ -1,0 +1,399 @@
+Require Import RocqOfRust.RocqOfRust.
+Require Import RocqOfRust.links.M.
+Require Import anza_xyz_solana_sdk.address.links.lib.
+Require Import anza_xyz_solana_sdk.program_error.links.lib.
+Require Import anza_xyz_solana_sdk.program_option.links.lib.
+Require Import anza_xyz_solana_sdk.program_pack.links.lib.
+Require Import solana_program_token.interface.state.
+
+(*
+  pub enum AccountState {
+      Uninitialized,
+      Initialized,
+      Frozen,
+  }
+*)
+Module AccountState.
+  Inductive t : Set :=
+  | Uninitialized
+  | Initialized
+  | Frozen.
+
+  Global Instance IsLink : Link t := {
+    Φ := Ty.path "spl_token_interface::state::AccountState";
+    φ x :=
+      match x with
+      | Uninitialized =>
+          Value.StructTuple "spl_token_interface::state::AccountState::Uninitialized" [] [] []
+      | Initialized =>
+          Value.StructTuple "spl_token_interface::state::AccountState::Initialized" [] [] []
+      | Frozen =>
+          Value.StructTuple "spl_token_interface::state::AccountState::Frozen" [] [] []
+      end
+  }.
+
+  Definition of_ty : OfTy.t (Ty.path "spl_token_interface::state::AccountState").
+  Proof. eapply OfTy.Make with (A := t); reflexivity. Defined.
+  Smpl Add apply of_ty : of_ty.
+
+  Lemma of_value_with_Uninitialized :
+    Value.StructTuple "spl_token_interface::state::AccountState::Uninitialized" [] [] [] =
+    φ Uninitialized.
+  Proof. reflexivity. Qed.
+  Definition of_value_Uninitialized :
+    OfValue.t (Value.StructTuple "spl_token_interface::state::AccountState::Uninitialized" [] [] []).
+  Proof. econstructor; apply of_value_with_Uninitialized. Defined.
+  Smpl Add apply of_value_Uninitialized : of_value.
+
+  Lemma of_value_with_Initialized :
+    Value.StructTuple "spl_token_interface::state::AccountState::Initialized" [] [] [] =
+    φ Initialized.
+  Proof. reflexivity. Qed.
+  Definition of_value_Initialized :
+    OfValue.t (Value.StructTuple "spl_token_interface::state::AccountState::Initialized" [] [] []).
+  Proof. econstructor; apply of_value_with_Initialized. Defined.
+  Smpl Add apply of_value_Initialized : of_value.
+
+  Lemma of_value_with_Frozen :
+    Value.StructTuple "spl_token_interface::state::AccountState::Frozen" [] [] [] =
+    φ Frozen.
+  Proof. reflexivity. Qed.
+  Definition of_value_Frozen :
+    OfValue.t (Value.StructTuple "spl_token_interface::state::AccountState::Frozen" [] [] []).
+  Proof. econstructor; apply of_value_with_Frozen. Defined.
+  Smpl Add apply of_value_Frozen : of_value.
+End AccountState.
+
+(*
+  pub struct Mint {
+      pub mint_authority: COption<Pubkey>,
+      pub supply: u64,
+      pub decimals: u8,
+      pub is_initialized: bool,
+      pub freeze_authority: COption<Pubkey>,
+  }
+*)
+Module Mint.
+  Record t : Set := {
+    mint_authority : COption.t Address.t;
+    supply : U64.t;
+    decimals : U8.t;
+    is_initialized : bool;
+    freeze_authority : COption.t Address.t;
+  }.
+
+  Global Instance IsLink : Link t := {
+    Φ := Ty.path "spl_token_interface::state::Mint";
+    φ x :=
+      Value.StructRecord "spl_token_interface::state::Mint" [] [] [
+        ("mint_authority", φ x.(mint_authority));
+        ("supply", φ x.(supply));
+        ("decimals", φ x.(decimals));
+        ("is_initialized", φ x.(is_initialized));
+        ("freeze_authority", φ x.(freeze_authority))
+      ];
+  }.
+
+  Definition of_ty : OfTy.t (Ty.path "spl_token_interface::state::Mint").
+  Proof. eapply OfTy.Make with (A := t); reflexivity. Defined.
+  Smpl Add apply of_ty : of_ty.
+
+  Lemma of_value_with
+    (mint_authority : COption.t Address.t) (mint_authority' : Value.t)
+    (supply : U64.t) (supply' : Value.t)
+    (decimals : U8.t) (decimals' : Value.t)
+    (is_initialized : bool) (is_initialized' : Value.t)
+    (freeze_authority : COption.t Address.t) (freeze_authority' : Value.t)
+    :
+    mint_authority' = φ mint_authority ->
+    supply' = φ supply ->
+    decimals' = φ decimals ->
+    is_initialized' = φ is_initialized ->
+    freeze_authority' = φ freeze_authority ->
+    Value.StructRecord "spl_token_interface::state::Mint" [] [] [
+      ("mint_authority", mint_authority');
+      ("supply", supply');
+      ("decimals", decimals');
+      ("is_initialized", is_initialized');
+      ("freeze_authority", freeze_authority')
+    ] = φ (Build_t mint_authority supply decimals is_initialized freeze_authority).
+  Proof. intros; subst; reflexivity. Qed.
+  Smpl Add apply of_value_with : of_value.
+
+  Module SubPointer.
+    Definition get_mint_authority : SubPointer.Runner.t t
+      (Pointer.Index.StructRecord "spl_token_interface::state::Mint" "mint_authority") :=
+    {|
+      SubPointer.Runner.projection x := Some x.(mint_authority);
+      SubPointer.Runner.injection x y := Some (x <| mint_authority := y |>);
+    |}.
+
+    Lemma get_mint_authority_is_valid :
+      SubPointer.Runner.Valid.t get_mint_authority.
+    Proof. now constructor. Qed.
+    Smpl Add apply get_mint_authority_is_valid : run_sub_pointer.
+
+    Definition get_supply : SubPointer.Runner.t t
+      (Pointer.Index.StructRecord "spl_token_interface::state::Mint" "supply") :=
+    {|
+      SubPointer.Runner.projection x := Some x.(supply);
+      SubPointer.Runner.injection x y := Some (x <| supply := y |>);
+    |}.
+
+    Lemma get_supply_is_valid :
+      SubPointer.Runner.Valid.t get_supply.
+    Proof. now constructor. Qed.
+    Smpl Add apply get_supply_is_valid : run_sub_pointer.
+
+    Definition get_decimals : SubPointer.Runner.t t
+      (Pointer.Index.StructRecord "spl_token_interface::state::Mint" "decimals") :=
+    {|
+      SubPointer.Runner.projection x := Some x.(decimals);
+      SubPointer.Runner.injection x y := Some (x <| decimals := y |>);
+    |}.
+
+    Lemma get_decimals_is_valid :
+      SubPointer.Runner.Valid.t get_decimals.
+    Proof. now constructor. Qed.
+    Smpl Add apply get_decimals_is_valid : run_sub_pointer.
+
+    Definition get_is_initialized : SubPointer.Runner.t t
+      (Pointer.Index.StructRecord "spl_token_interface::state::Mint" "is_initialized") :=
+    {|
+      SubPointer.Runner.projection x := Some x.(is_initialized);
+      SubPointer.Runner.injection x y := Some (x <| is_initialized := y |>);
+    |}.
+
+    Lemma get_is_initialized_is_valid :
+      SubPointer.Runner.Valid.t get_is_initialized.
+    Proof. now constructor. Qed.
+    Smpl Add apply get_is_initialized_is_valid : run_sub_pointer.
+
+    Definition get_freeze_authority : SubPointer.Runner.t t
+      (Pointer.Index.StructRecord "spl_token_interface::state::Mint" "freeze_authority") :=
+    {|
+      SubPointer.Runner.projection x := Some x.(freeze_authority);
+      SubPointer.Runner.injection x y := Some (x <| freeze_authority := y |>);
+    |}.
+
+    Lemma get_freeze_authority_is_valid :
+      SubPointer.Runner.Valid.t get_freeze_authority.
+    Proof. now constructor. Qed.
+    Smpl Add apply get_freeze_authority_is_valid : run_sub_pointer.
+  End SubPointer.
+End Mint.
+
+(*
+  pub struct Account {
+      pub mint: Pubkey,
+      pub owner: Pubkey,
+      pub amount: u64,
+      pub delegate: COption<Pubkey>,
+      pub state: AccountState,
+      pub is_native: COption<u64>,
+      pub delegated_amount: u64,
+      pub close_authority: COption<Pubkey>,
+  }
+*)
+Module Account.
+  Record t : Set := {
+    mint : Address.t;
+    owner : Address.t;
+    amount : U64.t;
+    delegate : COption.t Address.t;
+    state : AccountState.t;
+    is_native : COption.t U64.t;
+    delegated_amount : U64.t;
+    close_authority : COption.t Address.t;
+  }.
+
+  Global Instance IsLink : Link t := {
+    Φ := Ty.path "spl_token_interface::state::Account";
+    φ x :=
+      Value.StructRecord "spl_token_interface::state::Account" [] [] [
+        ("mint", φ x.(mint));
+        ("owner", φ x.(owner));
+        ("amount", φ x.(amount));
+        ("delegate", φ x.(delegate));
+        ("state", φ x.(state));
+        ("is_native", φ x.(is_native));
+        ("delegated_amount", φ x.(delegated_amount));
+        ("close_authority", φ x.(close_authority))
+      ];
+  }.
+
+  Definition of_ty : OfTy.t (Ty.path "spl_token_interface::state::Account").
+  Proof. eapply OfTy.Make with (A := t); reflexivity. Defined.
+  Smpl Add apply of_ty : of_ty.
+
+  Lemma of_value_with
+    (mint : Address.t) (mint' : Value.t)
+    (owner : Address.t) (owner' : Value.t)
+    (amount : U64.t) (amount' : Value.t)
+    (delegate : COption.t Address.t) (delegate' : Value.t)
+    (state : AccountState.t) (state' : Value.t)
+    (is_native : COption.t U64.t) (is_native' : Value.t)
+    (delegated_amount : U64.t) (delegated_amount' : Value.t)
+    (close_authority : COption.t Address.t) (close_authority' : Value.t)
+    :
+    mint' = φ mint ->
+    owner' = φ owner ->
+    amount' = φ amount ->
+    delegate' = φ delegate ->
+    state' = φ state ->
+    is_native' = φ is_native ->
+    delegated_amount' = φ delegated_amount ->
+    close_authority' = φ close_authority ->
+    Value.StructRecord "spl_token_interface::state::Account" [] [] [
+      ("mint", mint');
+      ("owner", owner');
+      ("amount", amount');
+      ("delegate", delegate');
+      ("state", state');
+      ("is_native", is_native');
+      ("delegated_amount", delegated_amount');
+      ("close_authority", close_authority')
+    ] = φ (Build_t mint owner amount delegate state is_native delegated_amount close_authority).
+  Proof. intros; subst; reflexivity. Qed.
+  Smpl Add apply of_value_with : of_value.
+
+  Module SubPointer.
+    Definition get_mint : SubPointer.Runner.t t
+      (Pointer.Index.StructRecord "spl_token_interface::state::Account" "mint") :=
+    {|
+      SubPointer.Runner.projection x := Some x.(mint);
+      SubPointer.Runner.injection x y := Some (x <| mint := y |>);
+    |}.
+
+    Lemma get_mint_is_valid :
+      SubPointer.Runner.Valid.t get_mint.
+    Proof. now constructor. Qed.
+    Smpl Add apply get_mint_is_valid : run_sub_pointer.
+
+    Definition get_owner : SubPointer.Runner.t t
+      (Pointer.Index.StructRecord "spl_token_interface::state::Account" "owner") :=
+    {|
+      SubPointer.Runner.projection x := Some x.(owner);
+      SubPointer.Runner.injection x y := Some (x <| owner := y |>);
+    |}.
+
+    Lemma get_owner_is_valid :
+      SubPointer.Runner.Valid.t get_owner.
+    Proof. now constructor. Qed.
+    Smpl Add apply get_owner_is_valid : run_sub_pointer.
+
+    Definition get_amount : SubPointer.Runner.t t
+      (Pointer.Index.StructRecord "spl_token_interface::state::Account" "amount") :=
+    {|
+      SubPointer.Runner.projection x := Some x.(amount);
+      SubPointer.Runner.injection x y := Some (x <| amount := y |>);
+    |}.
+
+    Lemma get_amount_is_valid :
+      SubPointer.Runner.Valid.t get_amount.
+    Proof. now constructor. Qed.
+    Smpl Add apply get_amount_is_valid : run_sub_pointer.
+
+    Definition get_delegate : SubPointer.Runner.t t
+      (Pointer.Index.StructRecord "spl_token_interface::state::Account" "delegate") :=
+    {|
+      SubPointer.Runner.projection x := Some x.(delegate);
+      SubPointer.Runner.injection x y := Some (x <| delegate := y |>);
+    |}.
+
+    Lemma get_delegate_is_valid :
+      SubPointer.Runner.Valid.t get_delegate.
+    Proof. now constructor. Qed.
+    Smpl Add apply get_delegate_is_valid : run_sub_pointer.
+
+    Definition get_state : SubPointer.Runner.t t
+      (Pointer.Index.StructRecord "spl_token_interface::state::Account" "state") :=
+    {|
+      SubPointer.Runner.projection x := Some x.(state);
+      SubPointer.Runner.injection x y := Some (x <| state := y |>);
+    |}.
+
+    Lemma get_state_is_valid :
+      SubPointer.Runner.Valid.t get_state.
+    Proof. now constructor. Qed.
+    Smpl Add apply get_state_is_valid : run_sub_pointer.
+
+    Definition get_is_native : SubPointer.Runner.t t
+      (Pointer.Index.StructRecord "spl_token_interface::state::Account" "is_native") :=
+    {|
+      SubPointer.Runner.projection x := Some x.(is_native);
+      SubPointer.Runner.injection x y := Some (x <| is_native := y |>);
+    |}.
+
+    Lemma get_is_native_is_valid :
+      SubPointer.Runner.Valid.t get_is_native.
+    Proof. now constructor. Qed.
+    Smpl Add apply get_is_native_is_valid : run_sub_pointer.
+
+    Definition get_delegated_amount : SubPointer.Runner.t t
+      (Pointer.Index.StructRecord "spl_token_interface::state::Account" "delegated_amount") :=
+    {|
+      SubPointer.Runner.projection x := Some x.(delegated_amount);
+      SubPointer.Runner.injection x y := Some (x <| delegated_amount := y |>);
+    |}.
+
+    Lemma get_delegated_amount_is_valid :
+      SubPointer.Runner.Valid.t get_delegated_amount.
+    Proof. now constructor. Qed.
+    Smpl Add apply get_delegated_amount_is_valid : run_sub_pointer.
+
+    Definition get_close_authority : SubPointer.Runner.t t
+      (Pointer.Index.StructRecord "spl_token_interface::state::Account" "close_authority") :=
+    {|
+      SubPointer.Runner.projection x := Some x.(close_authority);
+      SubPointer.Runner.injection x y := Some (x <| close_authority := y |>);
+    |}.
+
+    Lemma get_close_authority_is_valid :
+      SubPointer.Runner.Valid.t get_close_authority.
+    Proof. now constructor. Qed.
+    Smpl Add apply get_close_authority_is_valid : run_sub_pointer.
+  End SubPointer.
+End Account.
+
+(* impl Account *)
+Module Impl_Account.
+  Definition Self : Set := Account.t.
+
+  (* pub fn is_frozen(&self) -> bool *)
+  Instance run_is_frozen
+      (self : Ref.t Pointer.Kind.Ref Self) :
+    Run.Trait state.Impl_spl_token_interface_state_Account.is_frozen [] [] [φ self]
+      bool.
+  Proof.
+    constructor.
+    run_symbolic.
+  Admitted.
+  Global Opaque run_is_frozen.
+
+  (* pub fn is_native(&self) -> bool *)
+  Instance run_is_native
+      (self : Ref.t Pointer.Kind.Ref Self) :
+    Run.Trait state.Impl_spl_token_interface_state_Account.is_native [] [] [φ self]
+      bool.
+  Proof.
+    constructor.
+    run_symbolic.
+  Admitted.
+  Global Opaque run_is_native.
+End Impl_Account.
+Export (hints) Impl_Account.
+
+(* impl Pack for Mint *)
+Module Impl_Pack_for_Mint.
+  Instance run : Pack.Run Mint.t.
+  Admitted.
+End Impl_Pack_for_Mint.
+Export Impl_Pack_for_Mint.
+
+(* impl Pack for Account *)
+Module Impl_Pack_for_Account.
+  Instance run : Pack.Run Account.t.
+  Admitted.
+End Impl_Pack_for_Account.
+Export Impl_Pack_for_Account.
