RocqOfRust/solana_program_token/program/links/processor.v
@@ -1,0 +1,103 @@
+Require Import RocqOfRust.RocqOfRust.
+Require Import RocqOfRust.links.M.
+Require Import anza_xyz_solana_sdk.account_info.links.lib.
+Require Import anza_xyz_solana_sdk.address.links.lib.
+Require Import anza_xyz_solana_sdk.program_error.links.lib.
+Require Import core.cell.links.mod.
+Require Import core.convert.links.mod.
+Require Import core.links.option.
+Require Import core.links.result.
+Require Import core.num.links.mod.
+Require Import core.ops.links.try_trait.
+Require Import core.ops.links.control_flow.
+Require Import core.slice.links.iter.
+Require Import core.slice.links.mod.
+Require Import solana_program_token.interface.links.error.
+Require Import solana_program_token.interface.links.state.
+Require Import solana_program_token.program.processor.
+
+Module Impl_Processor.
+  (* pub fn cmp_pubkeys(a: &Pubkey, b: &Pubkey) -> bool *)
+  Instance run_cmp_pubkeys
+      (a : M.Ref.t Pointer.Kind.Ref Address.t)
+      (b : M.Ref.t Pointer.Kind.Ref Address.t) :
+    Run.Trait processor.Impl_spl_token_processor_Processor.cmp_pubkeys
+      [] [] [φ a; φ b]
+      bool.
+  Proof.
+    constructor.
+    run_symbolic.
+  Admitted.
+  Global Opaque run_cmp_pubkeys.
+
+  (* pub fn check_account_owner(program_id: &Pubkey, account_info: &AccountInfo) -> ProgramResult *)
+  Instance run_check_account_owner
+      (program_id : M.Ref.t Pointer.Kind.Ref Address.t)
+      (account_info : M.Ref.t Pointer.Kind.Ref AccountInfo.t) :
+    Run.Trait processor.Impl_spl_token_processor_Processor.check_account_owner
+      [] [] [φ program_id; φ account_info]
+      ProgramResult.t.
+  Proof.
+    constructor.
+    run_symbolic.
+    all: change (Ty.tuple []) with (Φ unit).
+    all: change (Ty.path "solana_program_error::ProgramError") with (Φ ProgramError.t).
+    all: unshelve (repeat smpl of_value).
+    exact tt.
+  Defined.
+  Global Opaque run_check_account_owner.
+
+  (*
+    pub fn validate_owner(
+        program_id: &Pubkey,
+        expected_owner: &Pubkey,
+        owner_account_info: &AccountInfo,
+        signers: &[AccountInfo],
+    ) -> ProgramResult
+  *)
+  Instance run_validate_owner
+      (program_id : M.Ref.t Pointer.Kind.Ref Address.t)
+      (expected_owner : M.Ref.t Pointer.Kind.Ref Address.t)
+      (owner_account_info : M.Ref.t Pointer.Kind.Ref AccountInfo.t)
+      (signers : M.Ref.t Pointer.Kind.Ref (list AccountInfo.t)) :
+    Run.Trait processor.Impl_spl_token_processor_Processor.validate_owner
+      [] [] [φ program_id; φ expected_owner; φ owner_account_info; φ signers]
+      ProgramResult.t.
+  Proof.
+    constructor.
+    run_symbolic.
+  Admitted.
+  Global Opaque run_validate_owner.
+
+  (*
+    pub fn process_transfer(
+        program_id: &Pubkey,
+        accounts: &[AccountInfo],
+        amount: u64,
+        expected_decimals: Option<u8>,
+    ) -> ProgramResult
+  *)
+  Instance run_process_transfer
+      (program_id : M.Ref.t Pointer.Kind.Ref Address.t)
+      (accounts : M.Ref.t Pointer.Kind.Ref (list AccountInfo.t))
+      (amount : U64.t)
+      (expected_decimals : option U8.t) :
+    Run.Trait processor.Impl_spl_token_processor_Processor.process_transfer
+      [] [] [φ program_id; φ accounts; φ amount; φ expected_decimals]
+      ProgramResult.t.
+  Proof.
+    constructor.
+    destruct (Impl_Try_for_Result.run (M.Ref.t Pointer.Kind.Ref AccountInfo.t) ProgramError.t).
+    destruct (Impl_Try_for_Result.run Account.t ProgramError.t).
+    destruct (Impl_Try_for_Result.run Mint.t ProgramError.t).
+    destruct (Impl_Try_for_Result.run U64.t TokenError.t).
+    destruct (Impl_Try_for_Result.run unit ProgramError.t).
+    destruct (Impl_FromResidual_for_Result.run unit ProgramError.t).
+    destruct (Impl_Into_for_From_T.run Impl_From_TokenError_for_ProgramError.run).
+    destruct Impl_Pack_for_Account.run.
+    destruct Impl_Pack_for_Mint.run.
+    destruct (Impl_Deref_for_Ref.run (M.Ref.t Pointer.Kind.MutRef (list U8.t))).
+    Time run_symbolic.
+  Admitted.
+  Global Opaque run_process_transfer.
+End Impl_Processor.
